\documentclass[10pt]{article}
\usepackage[linespread=1.18]{ctex}
\usepackage[ruled,vlined]{algorithm2e}
\usepackage{algpseudocode}
\usepackage{amsmath}
\usepackage{amsthm}
\usepackage{graphicx}
\usepackage{subfigure}
\usepackage{float}
\usepackage{amsmath }
\usepackage{amsfonts }
\usepackage{pdfpages}
\usepackage{epsfig}
\usepackage{graphicx}
\usepackage{arydshln}
\usepackage{verbatim}
\usepackage{subfigure}
\usepackage{enumerate}
\usepackage{rotating}
\usepackage{threeparttable}
\usepackage{caption}
\usepackage{epsfig}
\usepackage{cite}
\usepackage{geometry}
\geometry{a4paper,scale=0.9}

\newcommand{\cukai}{\CJKfamily{cukai}}
\newtheorem{myprob}{Problem}
\newtheorem{mythm}{Theorem}

\usepackage{multicol}

\title{\Huge\textbf{Discrete Math (Honor) 2021-Fall Homework-3}}

\author{\cukai\zihao{3}\textbf{王凯灵521030910356}
}


\date{}
\begin{document}
	\maketitle

\noindent\textbf{Solution 1.}
\begin{enumerate}
	\item
	First suppose R is false. Let's turn it into a CNF:

	\centerline {$ (P\vee Q)\wedge (\neg P \vee R)\wedge (\neg Q \vee R)\wedge \neg R$}

	Build resolve set S:

	\centerline {$ S =  \{P\vee Q,\neg P \vee R,\neg Q \vee R, \neg R\} $}

	Resolution:

	\normalsize{\textcircled{\footnotesize{1}}}~$P \vee Q$

	\normalsize{\textcircled{\footnotesize{2}}}~$\neg P \vee Q$

	\normalsize{\textcircled{\footnotesize{3}}}~$\neg Q \vee R$

	\normalsize{\textcircled{\footnotesize{4}}}~$\neg R$

	\normalsize{\textcircled{\footnotesize{5}}}~$Q \vee R$

	\normalsize{\textcircled{\footnotesize{6}}}~$R$

	\normalsize{\textcircled{\footnotesize{7}}}~Contradiction.

	\vspace{-5pt}
	\item
	CNF:

	\centerline{$ (\neg S \vee \neg Q)\wedge (\neg P \vee Q)\wedge (R\vee S)\wedge (\neg R \vee \neg Q)\wedge P$}

	\centerline{$S=\{\neg S \vee \neg Q,\neg P \vee Q,R\vee S,\neg R \vee \neg Q, P,\neg S\vee \neg P,S \vee \neg Q\}$}
	Resolution:

	\normalsize{\textcircled{\footnotesize{1}}}~$P$

	\normalsize{\textcircled{\footnotesize{2}}}~$\neg S \vee \neg P$

	\normalsize{\textcircled{\footnotesize{3}}}~$\neg S$

	\normalsize{\textcircled{\footnotesize{4}}}~$S \vee \neg Q$

	\normalsize{\textcircled{\footnotesize{5}}}~$\neg Q$

	\normalsize{\textcircled{\footnotesize{6}}}~$\neg P \vee Q$

	\normalsize{\textcircled{\footnotesize{7}}}~$\neg P$

	\normalsize{\textcircled{\footnotesize{8}}}~Contradiction.

	\vspace{-5pt}
	\item
	CNF:

	\centerline{$(\neg P\vee Q)\wedge (\neg Q\vee R)\wedge \neg R \wedge P$}

	\centerline{$S=\{\neg P\vee Q,\neg Q\vee R, \neg R, P\}$}

	Resolution:

	\normalsize{\textcircled{\footnotesize{1}}}~$P$

	\normalsize{\textcircled{\footnotesize{2}}}~$\neg P \vee Q$

	\normalsize{\textcircled{\footnotesize{3}}}~$Q$

	\normalsize{\textcircled{\footnotesize{4}}}~$\neg Q\vee R$

	\normalsize{\textcircled{\footnotesize{5}}}~$R$

	\normalsize{\textcircled{\footnotesize{6}}}~$\neg R$

	\normalsize{\textcircled{\footnotesize{7}}}~Contradiction.
\end{enumerate}

\noindent\textbf{Solution 2.}

$D:all~people.Eq(x,y):x=y.Fri(x,y):x, y~are~firends.Lov(x,y):x~loves~y.Hat(x,y):x~hates~y.$

\begin{enumerate}
	\item
	$(\forall x)(\forall y)(\neg Eq(x,y)\rightarrow Lov(x,y))$
	\item
	$(\forall x)(Student(x)\wedge \neg Eq(x,Alice)\rightarrow Fri(x,Bob))$
	\item
	$(\forall x)(student(x)\wedge Talkable(x)\rightarrow Walkable(x))$
	\item
	$(\forall x)(Boy(x)\wedge Lov(x,Alice)\wedge (\forall y) Lov(Alice,y)\rightarrow Hat(x,y))$
	\item
	$(\forall x)(Boy(x)\wedge Lov(x,Alice)\wedge (\forall y) Lov(Cauchy,y)\wedge Eq(x,y) \rightarrow Hat(x,y))$
	\item
	$(\exists x)(Love(x,Alice)\wedge Hate(x,Bob)))$
	\item
	$(\exists x)(Love(x,Alice)\wedge (\forall y)(Love(y,Bob)\wedge Hate(x,y)))$

\end{enumerate}
	\begin{myprob}  (10 Points)\\ \upshape
		For each of the following formulae, determine   free variables and   bound variables in it and determine the scope of each quantifier. \vspace{-5pt}
		\begin{enumerate}
			\item
			$(\forall x)(P(x)\to Q(x,y))$\vspace{-5pt}
			\item
			$(\forall x)P(x,y)\to (\exists y)Q(x,y)$ \vspace{-5pt}
			\item
			$(\forall x)(\exists y)( P(x,y)\wedge Q(y,z)\vee (\exists x)R(x,y,z) )$\vspace{-5pt}
			\item
			$(\exists x)( P(x)\to Q(x) ) \to (\exists y)R(y) \to S(z)$\vspace{-5pt}
			\item
			$(\forall x)( P(x)\wedge (\exists y)Q(y))\vee((\forall x)P(x)\to Q(z))   $
		\end{enumerate}
	\end{myprob}

\noindent\textbf{Solution 3.}

\begin{enumerate}
	\item
	free variable:$y$

	bound variable:$x$

	the scope of $\forall x$ is $P(x)\to Q(x,y)$

	\item
	free variable: the first $y$ and the second $x$

	bound variable: the first $x$ and the second $y$

	the scope of $\forall x$ is $P(x,y)$,the scope of $\exists y$ is $Q(x,y)$

	\item
	free variable: $z$

	bound variable: $x$ and $y$

	the scope of $\forall x$ is $\exists y)( P(x,y)\wedge Q(y,z)\vee (\exists x)R(x,y,z)$

	the scope of $\exists y$ is $( P(x,y)\wedge Q(y,z)\vee (\exists x)R(x,y,z)$

	the scope of $\exists x$ is $R(x,y,z)$

	\item
	free variable: $z$

	bound variable: $x$ and $y$

	the scope of $\exists x$ is $P(x)\to Q(x)$

	the scope of $\exists y$ is $R(y)$

	\item
	free variable: $z$

	bound variable: $x$ and $y$

	the scope of the first $\forall x$ is $ P(x)\wedge (\exists y)Q(y)$

	the scope of $\exists y$ is $Q(y)$

	the scope of the second $\forall x$ is $P(x)$

\end{enumerate}



\end{document}
